almost finished TP

Interp.v
@@ -13,7 +13,32 @@ Require Import WhileBigStep.
 Require Import Lia.
 
 Fixpoint exec_prog (fuel: nat) (env: state) (i: stmt) : option state :=
-None.
+  match fuel with
+  | O => None
+  | S fuel' =>
+    match i with
+    | Skip => Some env
+    | Assign x e => Some (update_state env x ( eval_expr env e))
+    | Seq s1 s2 =>
+      match exec_prog fuel' env s1 with
+      | Some env' => exec_prog fuel' env' s2
+      | None => None
+      end 
+    | If c s1 s2 => 
+      if eval_cond env c
+      then exec_prog fuel' env s1
+      else exec_prog fuel' env s2
+    | While c I1 s => 
+      if eval_cond env c
+      then match exec_prog fuel' env s with
+           | Some env' => exec_prog fuel' env' (While c I1 s)
+           | None => None
+          end
+      else Some env
+    end
+  end.
+
+(* On définit un programme qui calcule la somme des entiers de 1 à 10. *)
 
 Definition p1 :=
   Seq
@@ -38,7 +63,35 @@ Compute
 Theorem exec_prog_bigstep:
   forall fuel s i s', exec_prog fuel s i = Some s' -> bigstep s i s'.
 Proof.
-Admitted.
+  induction fuel; intros s i s' Hexec.
+  - discriminate.
+  - destruct i.
+    + inversion Hexec. apply bigstep_skip.
+    + inversion Hexec. apply bigstep_assign.
+    + inversion Hexec. destruct (exec_prog fuel s i1) eqn:Hexec1.
+      * apply bigstep_seq with (env':=s0).
+        -- apply IHfuel. apply Hexec1.
+        -- apply IHfuel. apply H0.
+      * discriminate.
+    + destruct (eval_cond s c) eqn:Hcond.
+      * inversion Hexec. apply bigstep_if_true.
+        -- rewrite eval_cond_true. apply Hcond.
+        -- apply IHfuel. rewrite Hcond in H0. apply H0.
+      * inversion Hexec. apply bigstep_if_false.
+        -- rewrite eval_cond_false. apply Hcond.
+        -- apply IHfuel. rewrite Hcond in H0. apply H0.
+    + destruct (eval_cond s c) eqn:Hcond.
+      * destruct (exec_prog fuel s i) eqn:Hexec1.
+        -- inversion Hexec. rewrite Hcond in H0. apply bigstep_while_true with (env':=s0).
+          ++ rewrite eval_cond_true. apply Hcond.
+          ++ apply IHfuel. apply Hexec1.
+          ++ apply IHfuel. rewrite Hexec1 in H0. apply H0.
+        -- inversion Hexec. rewrite Hcond in H0. rewrite Hexec1 in H0. discriminate.
+      * inversion Hexec. rewrite Hcond in H0. inversion H0. apply bigstep_while_false.
+        rewrite eval_cond_false. rewrite <- H1. apply Hcond.
+Qed.
+
+
 
 Lemma exec_prog_more_fuel:
   forall f s i s',
@@ -46,12 +99,74 @@ Lemma exec_prog_more_fuel:
   -> forall f', f' >= f
   -> exec_prog f' s i = Some s'.
 Proof.
-Admitted.
+  intros f. induction f; intros.
+  - discriminate.
+  - destruct f'.
+    + lia.
+    + destruct i.
+      * inversion H. reflexivity.
+      * inversion H. reflexivity.
+      * simpl. simpl in H. destruct (exec_prog f s i1) eqn:Hexec1.
+        -- apply IHf with (f':=f') in Hexec1.
+            ++ rewrite Hexec1. apply IHf with (f':=f') in H.
+                ** apply H.
+                ** lia.
+            ++ lia.
+        -- discriminate.
+      * simpl. simpl in H. destruct (eval_cond s c) eqn:Hcond.
+        -- apply IHf with (f':=f') in H.
+            ++ rewrite H. reflexivity.
+            ++ lia.
+        -- apply IHf with (f':=f') in H. 
+            ++ rewrite H. reflexivity.
+            ++ lia.
+      * simpl. simpl in H. destruct (eval_cond s c) eqn:Hcond.
+        -- destruct (exec_prog f s i) eqn:Hexec1.
+            ++ apply IHf with (f':=f') in Hexec1.
+                ** rewrite Hexec1. apply IHf with (f':=f') in H.
+                    --- apply H.
+                    --- lia.
+                ** lia.
+            ++ discriminate.
+        -- apply H.
+Qed.
 
 Theorem bigstep_exec_prog:
   forall s i s',
   bigstep s i s'
   -> exists fuel, exec_prog fuel s i = Some s'.
 Proof.
-Admitted.
+  intros s i s' Hbigstep.
+  induction Hbigstep.
+  - exists 1. reflexivity.
+  - exists 1. reflexivity.
+  - destruct IHHbigstep1 as [fuel1 H1].
+    destruct IHHbigstep2 as [fuel2 H2].
+    exists (S (max fuel1 fuel2)). simpl. rewrite exec_prog_more_fuel with (f:=fuel1) (s':=env').
+    + rewrite exec_prog_more_fuel with (f:=fuel2) (s':=env'').
+      * reflexivity.
+      * apply H2.
+      * lia.
+    + apply H1.
+    + lia.
+  - destruct IHHbigstep as [fuel1 H1].
+    exists (S fuel1). simpl. rewrite H1. apply eval_cond_true in H. rewrite H. reflexivity.
+  - destruct IHHbigstep as [fuel1 H1].
+    exists (S fuel1). simpl. rewrite H1. apply eval_cond_false in H. rewrite H. reflexivity.
+  - destruct IHHbigstep1 as [fuel1 H1].
+    destruct IHHbigstep2 as [fuel2 H2].
+    exists (S (max fuel1 fuel2)). simpl. apply eval_cond_true in H. rewrite H.
+    + destruct (exec_prog fuel1 env s) eqn:Hexec1.
+      * rewrite exec_prog_more_fuel with (f:=fuel1) (s':=env').
+        -- rewrite exec_prog_more_fuel with (f:=fuel2) (s':=env'').
+            ++ reflexivity.
+            ++ apply H2.
+            ++ lia.
+        -- rewrite <- H1. apply Hexec1.
+        -- lia.
+      * discriminate.
+  - exists 1. simpl. apply eval_cond_false in H. rewrite H. reflexivity.
+Qed.
+
+     
 
