Equiv.v
@@ -11,6 +11,9 @@ Open Scope string_scope.
 Require Import While Tactics.
 Require Import WhileSmallStep WhileBigStep.
 
+Print star.
+Print step.
+
 Lemma star_seq:
   forall s1 env1 env2,
   star s1 env1 Skip env2
@@ -20,13 +23,44 @@ Lemma star_seq:
 Proof.
   intros s1 env1 env2 Hstar.
   dependent induction Hstar; simpl; intros.
-Admitted.
+  - eapply star_step.
+    + eapply step_seq_skip.
+    + apply H.
+  - eapply star_step.
+    + eapply step_seq. apply H.
+    + apply IHHstar. reflexivity. apply H0.
+Qed. 
+
 
 
 Theorem bigstep_star:
   forall i env env', bigstep env i env' -> star i env Skip env'.
 Proof.
-Admitted.
+  intros i env env' Hbigstep. induction Hbigstep.
+  - apply star_refl.
+  - eapply star_step.
+    + apply step_assign.
+    + apply star_refl.
+  - eapply star_seq.
+    + apply IHHbigstep1.
+    + apply IHHbigstep2.
+  - eapply star_step.
+    + apply step_if_true. apply H.
+    + apply IHHbigstep.
+  - eapply star_step.
+    + apply step_if_false. apply H.
+    + apply IHHbigstep.
+  - eapply star_step.
+    + apply step_while_true. apply H.
+    + eapply star_seq.
+      * apply IHHbigstep1.
+      * apply IHHbigstep2.
+  - eapply star_step.
+    + apply step_while_false. apply H.
+    + apply star_refl.
+Qed.
+
+Print bigstep.
 
 Lemma step_bigstep:
   forall i env i' env',
@@ -35,11 +69,36 @@ Lemma step_bigstep:
       bigstep env' i' env'' ->
       bigstep env i env''.
 Proof.
-Admitted.
-
+  intros i env i' env' Hstep. induction Hstep; intros.
+  - inversion H. eapply bigstep_assign.
+  - eapply bigstep_if_true.
+    + apply H.
+    + apply H0.
+  - eapply bigstep_if_false.
+    + apply H.
+    + apply H0.
+  - inversion H0. subst. eapply bigstep_while_true.
+    + apply H.
+    + apply H4.
+    + apply H6.
+  - inversion H0. subst. eapply bigstep_while_false. apply H.
+  - inversion H. subst. eapply bigstep_seq.
+    + apply IHHstep. apply H3.
+    + apply H5.
+  - econstructor. 
+    + econstructor.
+    + apply H.
+Qed.
 Theorem star_bigstep:
   forall i env env', star i env Skip env' -> bigstep env i env'.
 Proof.
-Admitted.
+  intros i env env' Hstar. dependent induction Hstar.
+  - econstructor.
+  - eapply step_bigstep.
+    + apply H.
+    + apply IHHstar. auto.
+Qed.
+  
+
 
 
